messageInvariantPrototypes/paxos/decentralized/hosts.dfy
@@ -1,4 +1,4 @@
-include "types.dfy"
+include "../types.dfy"
 
 
 /***************************************************************************************
@@ -6,6 +6,7 @@ include "types.dfy"
 ***************************************************************************************/
 
 module LeaderHost {
+  import opened MonotonicityLibrary
   import opened UtilitiesLibrary
   import opened Types
 
@@ -17,10 +18,41 @@ module LeaderHost {
   }
 
   datatype Variables = Variables(
-    receivedPromises: set<AcceptorId>,
-    value: Value, 
-    highestHeardBallot: Option<LeaderId>
-  )
+    receivedPromisesAndValue: MonotonicPromisesAndValue,
+    highestHeardBallot: MonotonicNatOption  // holds LeaderId
+  ) {
+
+    ghost predicate WF(c: Constants) {
+      receivedPromisesAndValue.f == c.f
+    }
+
+    // My highestHeardBallot >= b
+    ghost predicate HeardAtLeast(b: LeaderId) {
+      highestHeardBallot.MNSome? && highestHeardBallot.value >= b
+    }
+    
+    // My highestHeardBallot < b
+    ghost predicate HeardAtMost(b: LeaderId) {
+      highestHeardBallot.MNNone? || highestHeardBallot.value < b
+    }
+
+    ghost predicate CanPropose(c: Constants) {
+      && |receivedPromisesAndValue.promises| >= c.f+1
+    }
+
+    ghost predicate CanProposeV(c: Constants, val: Value) {
+      && CanPropose(c)
+      && receivedPromisesAndValue.value == val
+    }
+
+    ghost function Value() : Value {
+      receivedPromisesAndValue.value
+    }
+
+    ghost function ReceivedPromises() : set<AcceptorId> {
+      receivedPromisesAndValue.promises
+    }
+  } // end datatype Variables (Leader)
 
   ghost predicate GroupWFConstants(grp_c: seq<Constants>, f: nat) {
     && 0 < |grp_c|
@@ -32,6 +64,7 @@ module LeaderHost {
     && 0 < f
     && GroupWFConstants(grp_c, f)
     && |grp_v| == |grp_c|
+    && (forall i | 0 <= i < |grp_c| :: grp_v[i].WF(grp_c[i]))
   }
 
   ghost predicate GroupInit(grp_c: seq<Constants>, grp_v: seq<Variables>, f: nat) 
@@ -41,9 +74,8 @@ module LeaderHost {
   }
 
   ghost predicate Init(c: Constants, v: Variables) {
-    && v.receivedPromises == {}
-    && v.value == c.preferredValue
-    && v.highestHeardBallot == None
+    && v.receivedPromisesAndValue == PV({}, c.preferredValue, c.f)
+    && v.highestHeardBallot == MNNone
   }
 
   datatype Step =
@@ -53,61 +85,79 @@ module LeaderHost {
   {
     match step
       case PrepareStep => NextPrepareStep(c, v, v', msgOps)
-      case ReceiveStep => NextReceiveStep(c, v, v', msgOps)
+      case ReceiveStep => NextReceivePromiseStep(c, v, v', msgOps)
       case ProposeStep => NextProposeStep(c, v, v', msgOps)
       case StutterStep => NextStutterStep(c, v, v', msgOps)
   }
 
   ghost predicate NextPrepareStep(c: Constants, v: Variables, v': Variables, msgOps: MessageOps) {
     && msgOps.recv.None?
-    && msgOps.send == Some(Prepare(c.id))
+    && msgOps.send.Some?
+    && SendPrepare(c, v, v', msgOps.send.value)
+  }
+
+  // Send predicate
+  ghost predicate SendPrepare(c: Constants, v: Variables, v': Variables, msg: Message) {
+    // enabling conditions
+    && true
+    // send message and update v'
+    && msg == Prepare(c.id)
     && v' == v
   }
 
-  ghost predicate NextReceiveStep(c: Constants, v: Variables, v': Variables, msgOps: MessageOps) {
+  ghost predicate NextReceivePromiseStep(c: Constants, v: Variables, v': Variables, msgOps: MessageOps) {
     && msgOps.recv.Some?
     && msgOps.send.None?
-    && match msgOps.recv.value
-      case Promise(bal, acc, vbOpt) => 
-        // Enabling condition that I don't yet have a quorum. Not a safety issue, but can
-        // probably simplify proof, preventing the leader from potentially equivocating
-        // on its proposed value after receiving extraneous straggling promises.
-        && |v.receivedPromises| <= c.f
-        && acc !in v.receivedPromises
-        && if bal == c.id then
-            var doUpdate := 
-              && vbOpt.Some? 
-              && (|| v.highestHeardBallot.None?
-                  || (v.highestHeardBallot.Some? && vbOpt.value.b > v.highestHeardBallot.value));
-            v' == v.(
-              receivedPromises := v.receivedPromises + {acc},
-              value :=  if doUpdate then vbOpt.value.v else v.value,
-              highestHeardBallot := if doUpdate then Some(vbOpt.value.b) else v.highestHeardBallot
+    && ReceivePromise(c, v, v', msgOps.recv.value)
+  }
+
+  // Receive predicate
+  ghost predicate ReceivePromise(c: Constants, v: Variables, v': Variables, msg: Message) {
+    && msg.Promise?
+    && var bal := msg.bal;
+    && var acc := msg.acc;
+    && var vbOpt := msg.vbOpt;
+    && bal == c.id  // message is meant for me
+    // Enabling condition that I don't yet have a quorum. Not a safety issue, but can
+    // probably simplify proof, preventing the leader from potentially equivocating
+    // on its proposed value after receiving extraneous straggling promises.
+    && |v.receivedPromisesAndValue.promises| <= c.f
+    && acc !in v.receivedPromisesAndValue.promises
+    && var doUpdate := 
+          && vbOpt.Some? 
+          && v.HeardAtMost(vbOpt.value.b);
+    v' == v.(
+              receivedPromisesAndValue := PV(v.receivedPromisesAndValue.promises + {acc}, if doUpdate then vbOpt.value.v else v.receivedPromisesAndValue.value, c.f),
+              highestHeardBallot := if doUpdate then MNSome(vbOpt.value.b) else v.highestHeardBallot
             )
-          else 
-            // this promise is not for me
-            NextStutterStep(c, v, v', msgOps)
-      case _ =>
-        NextStutterStep(c, v, v', msgOps)
+  }
+
+  // Receive predicate trigger
+  // First 2 arguments are mandatory. Second argument identifies target host. 
+  ghost predicate ReceivePromiseTrigger(c: Constants, v: Variables, acc: AcceptorId) {
+    && acc in v.receivedPromisesAndValue.promises
   }
 
   ghost predicate NextProposeStep(c: Constants, v: Variables, v': Variables, msgOps: MessageOps) {
     && msgOps.recv.None?
-    && |v.receivedPromises| >= c.f+1  // enabling condition
-    // Enabling condition that my hightest heard 
-    // is smaller than my own ballot. Not a safety issue, but can probably simplify proof.
-    // It is equivalent to being preempted
-    && (v.highestHeardBallot.None? || v.highestHeardBallot.value <= c.id)
-    
-    // Tony: This is a target for monotonic transformation -- it would allow me to say that
-    // Propose messages are from some value once held by the leader
-    && msgOps.send == Some(Propose(c.id, v.value))
+    && msgOps.send.Some?
+    && SendPropose(c, v, v', msgOps.send.value)
+  }
+
+  // Send predicate
+  ghost predicate SendPropose(c: Constants, v: Variables, v': Variables, msg: Message) {
+    // enabling conditions
+    && v.CanProposeV(c, v.receivedPromisesAndValue.value)
+    && v.HeardAtMost(c.id)
+    // send message and update v'
+    && msg == Propose(c.id, v.receivedPromisesAndValue.value)
     && v' == v
   }
 
   ghost predicate NextStutterStep(c: Constants, v: Variables, v': Variables, msgOps: MessageOps) {
     && v == v'
     && msgOps.send == None
+    && msgOps.recv == None
   }
 
   ghost predicate Next(c: Constants, v: Variables, v': Variables, msgOps: MessageOps)
@@ -122,6 +172,7 @@ module LeaderHost {
 ***************************************************************************************/
 
 module AcceptorHost {
+  import opened MonotonicityLibrary
   import opened UtilitiesLibrary
   import opened Types
 
@@ -131,15 +182,47 @@ module AcceptorHost {
     && c.id == id
   }
 
+  datatype PendingPrepare = Prepare(bal:LeaderId)
+
   datatype Variables = Variables(
-    pendingMsg: Option<Message>,
-    promised: Option<LeaderId>,
-    acceptedVB: Option<ValBal>
+    pendingPrepare: Option<PendingPrepare>,
+    promised: MonotonicNatOption,   // contains LeaderId
+    acceptedVB: MonotonicVBOption
   ) {
+
     ghost predicate WF() {
-      pendingMsg.Some? ==> (pendingMsg.value.Prepare? || pendingMsg.value.Propose?)
+      acceptedVB.MVBSome? ==> (promised.MNSome? && acceptedVB.value.b <= promised.value)
     }
-  }
+
+    ghost predicate HasAccepted(vb: ValBal) {
+      && acceptedVB.MVBSome?
+      && acceptedVB.value == vb
+    }
+
+    ghost predicate HasAcceptedValue(v: Value) {
+      && acceptedVB.MVBSome?
+      && acceptedVB.value.v == v
+    }
+
+    ghost predicate HasPromisedAtLeast(b: LeaderId) {
+      && promised.MNSome?
+      && b <= promised.value
+    }
+
+    ghost predicate HasPromised(b: LeaderId) {
+      && promised.MNSome?
+      && b == promised.value
+    }
+
+    ghost predicate HasAcceptedAtLeastBal(b: LeaderId) {
+      && acceptedVB.MVBSome?
+      && b <= acceptedVB.value.b
+    }
+
+    ghost predicate HasAcceptedAtMostBal(b: LeaderId) {
+      acceptedVB.MVBSome? ==> acceptedVB.value.b < b
+    }
+  } // end datatype Variables (acceptor)
 
   ghost predicate GroupWFConstants(grp_c: seq<Constants>) {
     && 0 < |grp_c|
@@ -150,7 +233,7 @@ module AcceptorHost {
   ghost predicate GroupWF(grp_c: seq<Constants>, grp_v: seq<Variables>, f: nat) {
     && GroupWFConstants(grp_c)
     && |grp_v| == |grp_c| == 2*f+1
-    && forall i | 0 <= i < |grp_v| :: grp_v[i].WF()
+    && (forall i | 0 <= i < |grp_c| :: grp_v[i].WF())
   }
 
   ghost predicate GroupInit(grp_c: seq<Constants>, grp_v: seq<Variables>, f: nat) 
@@ -160,79 +243,118 @@ module AcceptorHost {
   }
 
   ghost predicate Init(c: Constants, v: Variables) {
-    && v.promised == None
-    && v.acceptedVB == None
-    && v.pendingMsg == None
+    && v.promised == MNNone
+    && v.acceptedVB == MVBNone
+    && v.pendingPrepare == None
   }
 
   datatype Step =
-    ReceiveStep() | MaybePromiseStep() | MaybeAcceptStep() | StutterStep()
+    ReceivePrepareStep() 
+    | MaybePromiseStep() 
+    | MaybeAcceptStep() 
+    | BroadcastAcceptedStep() 
+    | StutterStep()
 
   ghost predicate NextStep(c: Constants, v: Variables, v': Variables, step: Step, msgOps: MessageOps)
   {
     match step
-      case ReceiveStep => NextReceiveStep(c, v, v', msgOps)
+      case ReceivePrepareStep => NextReceivePrepareStep(c, v, v', msgOps)
       case MaybePromiseStep => NextMaybePromiseStep(c, v, v', msgOps)
       case MaybeAcceptStep => NextMaybeAcceptStep(c, v, v', msgOps)
+      case BroadcastAcceptedStep => NextBroadcastAcceptedStep(c, v, v', msgOps)
       case StutterStep => NextStutterStep(c, v, v', msgOps)
   }
 
-  ghost predicate NextReceiveStep(c: Constants, v: Variables, v': Variables, msgOps: MessageOps) {
-    && v.pendingMsg.None?
+  ghost predicate NextReceivePrepareStep(c: Constants, v: Variables, v': Variables, msgOps: MessageOps) {
     && msgOps.recv.Some?
     && msgOps.send.None?
-    && match msgOps.recv.value
-        case Prepare(_) =>
-          v' == v.(pendingMsg := Some(msgOps.recv.value))
-        case Propose(bal, val) =>
-          v' == v.(pendingMsg := Some(msgOps.recv.value))
-        case _ =>
-          NextStutterStep(c, v, v', msgOps)
+    && msgOps.recv.value.Prepare?
+    && v.pendingPrepare.None?
+    && v' == v.(
+      pendingPrepare := Some(PendingPrepare.Prepare(msgOps.recv.value.bal))
+    )
   }
 
-  ghost predicate NextMaybePromiseStep(c: Constants, v: Variables, v': Variables, msgOps: MessageOps) {
+  ghost predicate NextMaybePromiseStep(c: Constants, v: Variables, v': Variables, msgOps: MessageOps)
+  {
     && msgOps.recv.None?
-    && v.pendingMsg.Some?
-    && v.pendingMsg.value.Prepare?
-    && var bal := v.pendingMsg.value.bal;
-    && var doPromise := v.promised.None? || (v.promised.Some? && v.promised.value < bal);
+    && v.pendingPrepare.Some?
+    && var bal := v.pendingPrepare.value.bal;
+    && var doPromise := v.promised.MNSome? ==> v.promised.value < bal;
     && if doPromise then
-          && v' == v.(
-            promised := Some(bal),
-            pendingMsg := None)
-          && msgOps.send == Some(Promise(bal, c.id, v.acceptedVB)) 
+          && msgOps.send.Some?
+          && SendPromise(c, v, v', msgOps.send.value)
         else
-          && v' == v.(pendingMsg := None)
+          && v' == v.(pendingPrepare := None)
           && msgOps.send == None
+  }
+
+  // Send predicate
+  ghost predicate SendPromise(c: Constants, v: Variables, v': Variables, msg: Message) {
+    // enabling conditions
+    && v.pendingPrepare.Some?
+    && var bal := v.pendingPrepare.value.bal;
+    && var doPromise := v.promised.MNSome? ==> v.promised.value < bal;
+    && doPromise
+    // send message and update v'
+    && v' == v.(
+            promised := MNSome(bal),
+            pendingPrepare := None)
+    && msg == Promise(bal, c.id, v.acceptedVB.ToOption())
   }
 
   ghost predicate NextMaybeAcceptStep(c: Constants, v: Variables, v': Variables, msgOps: MessageOps) {
-    && msgOps.recv.None?
-    && v.pendingMsg.Some?
-    && v.pendingMsg.value.Propose?
-    && var bal := v.pendingMsg.value.bal;
-    && var val := v.pendingMsg.value.val;
-    && var doAccept := v.promised.None? || (v.promised.Some? && v.promised.value <= bal);
+    && msgOps.recv.Some?
+    && msgOps.recv.value.Propose?
+    && v.pendingPrepare.None?
+    && var bal := msgOps.recv.value.bal;
+    && var val := msgOps.recv.value.val;
+    && var doAccept := (v.promised.MNSome? ==> v.promised.value <= bal);
     &&  if doAccept then
-          && v' == v.(
-                promised := Some(bal), 
-                acceptedVB := Some(VB(val, bal)),
-                pendingMsg := None)
           && msgOps.send == Some(Accept(VB(val, bal), c.id))
+          && v' == v.(
+                promised := MNSome(bal), 
+                acceptedVB := MVBSome(VB(val, bal)))
         else
-          && v' == v.(pendingMsg := None)
-          && msgOps.send == None
+          && v' == v
+          && msgOps.send.None?
+  }
+
+  ghost predicate NextBroadcastAcceptedStep(c: Constants, v: Variables, v': Variables, msgOps: MessageOps)
+  {
+    && msgOps.recv == None
+    && msgOps.send.Some?
+    && SendAccept(c, v, v', msgOps.send.value)
+  }
+
+  // Send predicate
+  ghost predicate SendAccept(c: Constants, v: Variables, v': Variables, msg: Message) {
+    // enabling conditions
+    && v.pendingPrepare.None?
+    && v.acceptedVB.MVBSome?
+    && v.promised == MNSome(v.acceptedVB.value.b)
+    // send message and update v'
+    && msg == Accept(v.acceptedVB.value, c.id)
+    && v' == v
   }
 
   ghost predicate NextStutterStep(c: Constants, v: Variables, v': Variables, msgOps: MessageOps) {
-    && v == v'
     && msgOps.send == None
+    && msgOps.recv == None
+    && v' == v
   }
 
   ghost predicate Next(c: Constants, v: Variables, v': Variables, msgOps: MessageOps)
   {
     exists step :: NextStep(c, v, v', step, msgOps)
   }
+
+  lemma UpdateReceiveAcceptedStep(c: Constants, v: Variables, v': Variables, 
+    step: Step, msgOps: MessageOps)
+    requires NextStep(c, v, v', step, msgOps)
+    requires !step.MaybeAcceptStep?
+    ensures v'.acceptedVB == v.acceptedVB
+  {}
 }  // end module AcceptorHost
 
 
@@ -253,8 +375,14 @@ module LearnerHost {
 
   datatype Variables = Variables(
     // maps ValBal to acceptors that accepted such pair
-    receivedAccepts: map<ValBal, set<AcceptorId>>
-  )
+    receivedAccepts: MonotonicReceivedAccepts,
+    learned: Option<Value>
+  ) {
+    
+    ghost predicate HasLearnedValue(v: Value) {
+      learned == Some(v)
+    }
+  } // end datatype Variables (Learner)
 
   ghost predicate GroupWFConstants(grp_c: seq<Constants>, f: nat) {
     && 0 < |grp_c|
@@ -275,7 +403,8 @@ module LearnerHost {
   }
 
   ghost predicate Init(c: Constants, v: Variables) {
-    v.receivedAccepts == map[]
+    && v.receivedAccepts == RA(map[])
+    && v.learned == None
   }
 
   datatype Step =
@@ -284,46 +413,58 @@ module LearnerHost {
   ghost predicate NextStep(c: Constants, v: Variables, v': Variables, step: Step, msgOps: MessageOps)
   {
     match step
-      case ReceiveStep => NextReceiveStep(c, v, v', msgOps)
-      case LearnStep(vb) => NextLearnStep(c, v, v', msgOps, vb)
+      case ReceiveStep => NextReceiveAcceptStep(c, v, v', msgOps)
+      case LearnStep(vb) => NextLearnStep(c, v, v', vb, msgOps)
       case StutterStep => NextStutterStep(c, v, v', msgOps)
   }
 
-  function UpdateReceivedAccepts(receivedAccepts: map<ValBal, set<AcceptorId>>, 
-    vb: ValBal, acc: AcceptorId) : (out: map<ValBal, set<AcceptorId>>)
+  function UpdateReceivedAccepts(receivedAccepts: MonotonicReceivedAccepts, 
+    vb: ValBal, acc: AcceptorId) : (out: MonotonicReceivedAccepts)
     // Tony: ensures clauses are exactly how I can prove to the user, and tell dafny, that 
     // data structures annotated as monotonic actually are monotonic --- cool!
-    ensures vb in receivedAccepts ==> vb in out
-    ensures vb in receivedAccepts ==> |receivedAccepts[vb]| <= |out[vb]|
+    ensures vb in receivedAccepts.m ==> vb in out.m
+    ensures vb in receivedAccepts.m ==> |receivedAccepts.m[vb]| <= |out.m[vb]|
   {
-    if vb in receivedAccepts then 
-      UnionIncreasesCardinality(receivedAccepts[vb], {acc});
-      receivedAccepts[vb := receivedAccepts[vb] + {acc}]
+    if vb in receivedAccepts.m then 
+      UnionIncreasesCardinality(receivedAccepts.m[vb], {acc});
+      RA(receivedAccepts.m[vb := receivedAccepts.m[vb] + {acc}])
     else 
-      receivedAccepts[vb := {acc}]
+      RA(receivedAccepts.m[vb := {acc}])
   }
 
-  ghost predicate NextReceiveStep(c: Constants, v: Variables, v': Variables, msgOps: MessageOps) {
+  ghost predicate NextReceiveAcceptStep(c: Constants, v: Variables, v': Variables, msgOps: MessageOps) {
     && msgOps.recv.Some?
     && msgOps.send.None?
-    && match msgOps.recv.value
-      case Accept(vb, acc) => 
-        v' == Variables(UpdateReceivedAccepts(v.receivedAccepts, vb, acc))
-      case _ =>
-        NextStutterStep(c, v, v', msgOps)
+    && ReceiveAccept(c, v, v', msgOps.recv.value)
   }
 
-  ghost predicate NextLearnStep(c: Constants, v: Variables, v': Variables, msgOps: MessageOps, vb: ValBal) {
+  // Receive predicate
+  ghost predicate ReceiveAccept(c: Constants, v: Variables, v': Variables, msg: Message) {
+    && msg.Accept?
+    && v' == v.(
+      receivedAccepts := UpdateReceivedAccepts(v.receivedAccepts, msg.vb, msg.acc)
+    )
+  }
+
+  // Receive predicate trigger
+  // First 2 arguments are mandatory. Second argument identifies target host. 
+  ghost predicate ReceiveAcceptTrigger(c: Constants, v: Variables, acc: AcceptorId, vb: ValBal) {
+    && vb in v.receivedAccepts.m
+    && acc in v.receivedAccepts.m[vb]
+  }
+
+  ghost predicate NextLearnStep(c: Constants, v: Variables, v': Variables, vb: ValBal, msgOps: MessageOps) {
     && msgOps.recv.None?
-    && vb in v.receivedAccepts  // enabling
-    && |v.receivedAccepts[vb]| >= c.f + 1  // enabling
-    && msgOps.send == Some(Learn(c.id, vb.b, vb.v))
-    && v' == v  // local state unchanged
+    && msgOps.send.None?
+    && vb in v.receivedAccepts.m              // enabling
+    && |v.receivedAccepts.m[vb]| >= c.f + 1   // enabling
+    && v' == v.(learned := Some(vb.v))        // learn new value
   }
 
   ghost predicate NextStutterStep(c: Constants, v: Variables, v': Variables, msgOps: MessageOps) {
-    && v == v'
-    && msgOps.send == None
+    && msgOps.recv.None?
+    && msgOps.send.None?
+    && v' == v
   }
 
   ghost predicate Next(c: Constants, v: Variables, v': Variables, msgOps: MessageOps)
